\begin{proof}
Outline: the proof proceeds by finding a lower bound for the objective function in (\ref{proxG}) and then we show that the proposed solution achieves this lower bound.

First, note that the following is true for any $\bB$ and $\bV$,
\begin{align*}\label{eqn1}
\|\bB - \bV\|_F^2 &= \sum_{i=1}^p\|\bbeta_{i \a} - \bv_{i \a}\|^2 \\
 \geq \sum_{i=1}^p&(\|\bbeta_{i \a}\| - \|\bv_{i \a}\|)^2 = \|\tilde{\bbeta} - \tilde{\bv}\|^2
\end{align*}
where the inequality follows from reverse triangle inequality. 

Combining this with $G(\bB) = \Omega_{\bw}(\tilde{\bbeta})$, we have a lower bound on the objective function in ($\ref{proxG}$). For all $\bB \in \R^{p \times r}$
\begin{align*}
\frac{1}{2}\|\bB - \bV\|_F^2 + G(\bB)
&\geq \frac{1}{2} \|\textnormal{prox}_{\Omega_{\bw}}(\tilde{\bv}) -  \tilde{\bv}\|^2 + \Omega_{\bw}(\textnormal{prox}_{\Omega_{\bw}}(\tilde{\bv})) 
\end{align*}

Finally, we show that $\bB = \widehat \bV$ achieves this lower bound,
\begin{align*}
&\frac{1}{2}\|\widehat \bV - \bV\|_F^2 + G(\widehat \bV) \\
& = \frac{1}{2} \sum_{i = 1}^p \|(\textnormal{prox}_{\Omega_{\bw}}(\tilde{\bv}))_i \frac{\bv_{i \a}}{\|\bv_{i \a}\|} - \bv_{i \a}\|^2_2 + \Omega_{\bw}(\textnormal{prox}_{\Omega_{\bw}}(\tilde{\bv})) \\
 & = \frac{1}{2} \|\textnormal{prox}_{\Omega_{\bw}}(\tilde{\bv}) -  \tilde{\bv}\|^2_2 + \Omega_{\bw}(\textnormal{prox}_{\Omega_{\bw}}(\tilde{\bv})) 
\end{align*}
\end{proof}
